CertiGC/verif_do_generation.v
@@ -1,0 +1,6 @@
+Require Import RamifyCoq.CertiGC.gc_spec.
+
+Lemma body_do_scan: semax_body Vprog Gprog f_do_generation do_generation_spec.
+Proof.
+  start_function.
+Abort.
